QCP/SeparationLogic/sets/SetsClass.v
@@ -1,3 +1,0 @@
-Require Export SetsClass.SetsClass_AxiomFree.
-Require Export SetsClass.SetsDomain_Classic.
-
